WIP

src/Renaming.v
@@ -4,122 +4,65 @@ Require Import Var VarEquations.
 Inductive raw_renaming :=
   | raw_renaming_id : raw_renaming
   | raw_renaming_extend :
-      var -> raw_renaming -> option var -> raw_renaming.
+      var -> raw_renaming -> var -> raw_renaming.
 
-Fixpoint is_interesting_raw_renaming_extension v r vo :=
+Fixpoint is_interesting_raw_renaming_extension vl r vr :=
   match r with
-  | raw_renaming_id => negb (var_opt_var_eqb vo v)
-  | raw_renaming_extend v' r vo' =>
+  | raw_renaming_id => negb (var_eqb vl vr)
+  | raw_renaming_extend vl' r vr' =>
     is_interesting_raw_renaming_extension
-      (unshift_var v' v) r (unshift_var_opt vo' vo)
+      (unshift_var vl' vl) r (unshift_var vr' vr)
   end.
 
-Definition is_ordered_raw_renaming_var v r :=
+Fixpoint is_all_interesting_raw_renaming r :=
   match r with
   | raw_renaming_id => true
-  | raw_renaming_extend v' _ _ => is_less_equal_vars v v'
+  | raw_renaming_extend vl r' vr =>
+    andb
+      (is_interesting_raw_renaming_extension vl r' vr)
+      (is_all_interesting_raw_renaming r')
   end.
 
-Fixpoint is_normalized_raw_renaming r :=
-  match r with
-  | raw_renaming_id => true
-  | raw_renaming_extend v r vo =>
-    andb (is_ordered_raw_renaming_var v r)
-         (andb (is_interesting_raw_renaming_extension v r vo)
-               (is_normalized_raw_renaming r))
-  end.
-
-Definition normalized_raw_renaming r :=
-  if is_normalized_raw_renaming r then sUnit else sEmpty.
-
-Lemma normalized_raw_renaming_from_extend {v r vo} :
-  normalized_raw_renaming (raw_renaming_extend v r vo) ->
-  normalized_raw_renaming r.
+Lemma is_all_interesting_raw_renaming_from_extend {vl r vr} :
+  is_all_interesting_raw_renaming
+    (raw_renaming_extend vl r vr) = true ->
+  is_all_interesting_raw_renaming r = true.
 Proof.
-  unfold normalized_raw_renaming; cbn.
-  destruct (is_normalized_raw_renaming r); try easy.
-  rewrite !Bool.andb_false_r; easy.
+  destruct r; cbn;
+    try rewrite Bool.andb_true_iff; easy.
 Qed.
 
-Set Primitive Projections.
-Record renaming :=
-  mk_renaming {
-      r_raw : raw_renaming;
-      r_normalized : normalized_raw_renaming r_raw
-    }.
-Add Printing Constructor renaming.
-Unset Primitive Projections.
-
-Definition renaming_id : renaming :=
-  mk_renaming raw_renaming_id stt.
-
-Fixpoint raw_renaming_extend_boring v r vo :=
+Fixpoint raw_renaming_extend_boring vl r vr :=
   match r with
   | raw_renaming_id =>
-      if (var_opt_var_eqb vo v) then Some r
+      if (var_eqb vl vr) then Some r
       else None
-  | raw_renaming_extend v' r vo' =>
+  | raw_renaming_extend vl' r vr' =>
     match raw_renaming_extend_boring
-              (unshift_var v' v) r (unshift_var_opt vo' vo)
+              (unshift_var vl' vl) r (unshift_var vr' vr)
     with
     | None => None
     | Some r =>
       Some (raw_renaming_extend
-              (shift_var v v') r (shift_var_opt vo vo'))
+              (shift_var vl vl') r (shift_var vr vr'))
     end
   end.
 
-Lemma is_interesting_raw_renaming_extend_boring_none v r vo :
-  raw_renaming_extend_boring v r vo = None ->
-  is_interesting_raw_renaming_extension v r vo = true.
+Lemma is_interesting_raw_renaming_extend_boring_none vl r vr :
+  raw_renaming_extend_boring vl r vr = None ->
+  is_interesting_raw_renaming_extension vl r vr = true.
 Proof.
-  generalize dependent v.
-  generalize dependent vo.
-  induction r as [|v' r IHr vo']; cbn; intros vo v Heq.
-  - destruct (var_opt_var_eqb vo v); easy.
+  generalize dependent vl.
+  generalize dependent vr.
+  induction r as [|vl' r IHr vr']; cbn; intros vr vl Heq.
+  - destruct (var_eqb vl vr); easy.
   - apply IHr.
     destruct (raw_renaming_extend_boring
-                (unshift_var v' v) r (unshift_var_opt vo' vo));
+                (unshift_var vl' vl) r (unshift_var vr' vr));
       easy.
 Qed.
 
-Lemma is_normalized_raw_renaming_extend_boring_none
-      r v1 v2 vo1 vo2 :
-  is_normalized_raw_renaming (raw_renaming_extend v2 r vo2)
-  = true ->
-  raw_renaming_extend_boring
-    v1 (raw_renaming_extend v2 r vo2) vo1 = None ->
-  is_less_equal_vars v1 v2 = true ->
-  is_normalized_raw_renaming
-    (raw_renaming_extend v1 (raw_renaming_extend v2 r vo2) vo1)
-    = true.
-Proof.
-  intros Heq1 Heq2 Heq3; cbn in *.
-  rewrite Heq3, Heq1.
-  rewrite is_interesting_raw_renaming_extend_boring_none; try easy.
-  destruct (raw_renaming_extend_boring (unshift_var v2 v1) r
-             (unshift_var_opt vo2 vo1)); easy.
-Qed.
-
 (* TODO move to VarEquations.v *)
-Lemma var_opt_var_eqb_some_true v1 v2 :
-  var_opt_var_eqb (Some v1) v2 = true <-> v1 = v2.
-Proof.
-  unfold var_opt_var_eqb.
-  destruct (var_opt_var_dec (Some v1) v2).
-  - replace v1 with v2 by congruence; easy.
-  - split; intro; congruence.
-Qed.
-
-Lemma var_opt_var_eqb_some_false v1 v2 :
-  var_opt_var_eqb (Some v1) v2 = false <-> v1 <> v2.
-Proof.
-  unfold var_opt_var_eqb.
-  destruct (var_opt_var_dec (Some v1) v2).
-  - replace v1 with v2 by congruence; easy.
-  - split; intro; congruence.
-Qed.
-
 Lemma succ_var_injective v1 v2 :
   v1 <> v2 ->
   succ_var v1 <> succ_var v2.
@@ -140,196 +83,477 @@ Proof.
   rewrite Heq; easy.
 Qed.
 
-Lemma is_interesting_raw_renaming_extend_boring_shift_ind
-      r1 :
-  forall r2 v1 v2 v3 v4 vo1 vo2 vo3 vo4,
-  is_interesting_raw_renaming_extension v1 r1 vo1 = true ->
-  v3 = unshift_var v1 v2 ->
-  vo3 = unshift_var_opt vo1 vo2 ->
-  raw_renaming_extend_boring v3 r1 vo3 = Some r2 ->
-  v4 = shift_var v2 v1 ->
-  vo4 = shift_var_opt vo2 vo1 ->
-  is_interesting_raw_renaming_extension v4 r2 vo4 = true.
+Lemma var_eqb_false v1 v2 :
+  (var_eqb v1 v2 = false) <-> v1 <> v2.
 Proof.
-  induction r1 as [|v5 r1 IHr1 vo5]; cbn;
-    intros * Heq1 -> -> Heq2 -> ->.
+  unfold var_eqb.
+  destruct (var_dec v1 v2); easy.
+Qed.
+
+Lemma var_eqb_true v1 v2 :
+  (var_eqb v1 v2 = true) <-> v1 = v2.
+Proof.
+  unfold var_eqb.
+  destruct (var_dec v1 v2); easy.
+Qed.
+
+Lemma shift_neq vl1 vl2 vr1 vr2 :
+  vl1 <> vr1 ->
+  unshift_var vl1 vl2 = unshift_var vr1 vr2 ->
+  shift_var vl2 vl1 <> shift_var vr2 vr1.
+Proof.
+  intros Hneq Heq.
+  destruct (label_opt_dec (v_label_opt vl1) (v_label_opt vr1)).
+  - case_vars vl1 vl2; case_vars vr1 vr2; subst;
+      autorewrite with reduce_vars_beta in *;
+      try easy; try congruence;
+        solve [rewrite red_var_neq
+                by solve_v_label_opt_equation;
+               reduce_vars_beta; lia].
+  - apply mk_var_label_injective; reduce_vars_beta; easy.
+Qed.
+
+Lemma is_interesting_raw_renaming_extend_boring_some_ind
+      r1 :
+  forall r2 vl1 vl2 vr1 vr2,
+  is_interesting_raw_renaming_extension vl1 r1 vr1 = true ->
+  raw_renaming_extend_boring
+    (unshift_var vl1 vl2) r1 (unshift_var vr1 vr2) = Some r2 ->
+  is_interesting_raw_renaming_extension
+    (shift_var vl2 vl1) r2 (shift_var vr2 vr1) = true.
+Proof.
+  induction r1 as [|vl5 r1 IHr1 vr5]; cbn; intros * Heq1 Heq2.
   - destruct
-      (var_opt_var_eqb (unshift_var_opt vo1 vo2)
-                       (unshift_var v1 v2)) eqn:Heq3; try easy.
-    replace r2 with raw_renaming_id by congruence; cbn.
-    rewrite Bool.negb_true_iff in *.
-    destruct vo1 as [v3|], vo2 as [v4|]; cbn in *; try easy.
-    rewrite var_opt_var_eqb_some_false, var_opt_var_eqb_some_true
-      in *.
-    generalize Heq3.
-    case_vars v1 v2; case_vars v3 v4; try easy;
-      intros; subst; reduce_vars;
-        autorewrite with reduce_vars_beta in *;
-        try solve [rewrite red_var_neq
-                    by solve_v_label_opt_equation;
-                   reduce_vars_beta; lia];
-        try solve [apply mk_var_label_injective;
-                   solve_v_label_opt_equation];
-        solve [apply succ_var_injective; easy].
+      (var_eqb (unshift_var vl1 vl2) (unshift_var vr1 vr2))
+      eqn:Heq3; try easy.
+    injection Heq2 as <-; cbn.
+    rewrite Bool.negb_true_iff, var_eqb_false, var_eqb_true in *.
+    apply shift_neq; easy.
+  - destruct raw_renaming_extend_boring eqn:Heq3; try easy.
+    injection Heq2 as <-; cbn.
+    rewrite <- transpose_pops_reverse_middle.
+    rewrite transpose_pushes_reverse_middle.
+    apply IHr1; try easy.
+    rewrite transpose_pops_reverse_right.
+    rewrite transpose_pushes_reverse_left.
+    easy.
+Qed.
+
+Lemma is_interesting_raw_renaming_extend_boring_some vl r1 vr r2 :
+  is_all_interesting_raw_renaming r1 = true ->
+  raw_renaming_extend_boring vl r1 vr = Some r2 ->
+  is_all_interesting_raw_renaming r2 = true.
+Proof.
+  generalize dependent vl.
+  generalize dependent vr.
+  generalize dependent r2.
+  induction r1 as [|vl2 r1 ? vr2]; cbn;
+    intros r2 vr vl Heq1 Heq2.
+  - destruct var_eqb; try easy.
+    injection Heq2 as <-; easy.
+  - rewrite Bool.andb_true_iff in Heq1;
+      destruct Heq1 as [Heq1 Heq3].
+    destruct raw_renaming_extend_boring eqn:Heq4; try easy.
+    injection Heq2 as <-; cbn.
+    rewrite Bool.andb_true_iff; split.
+    + apply is_interesting_raw_renaming_extend_boring_some_ind
+        with (r1 := r1); easy.
+    + apply IHr1
+        with (vl := unshift_var vl2 vl) (vr := unshift_var vr2 vr);
+        easy.
+Qed.
+
+Definition interesting_raw_renaming_extend vl r vr :=
+  match raw_renaming_extend_boring vl r vr with
+  | Some r => r
+  | None => raw_renaming_extend vl r vr
+  end.
+
+Lemma is_all_interesing_raw_renaming_extend vl r vr :
+  is_all_interesting_raw_renaming r = true ->
+  is_all_interesting_raw_renaming
+    (interesting_raw_renaming_extend vl r vr) = true.
+Proof.
+  intro Heq1; unfold interesting_raw_renaming_extend.
+  destruct (raw_renaming_extend_boring vl r vr) eqn:Heq2; cbn.
+  - apply is_interesting_raw_renaming_extend_boring_some
+      in Heq2; easy.
+  - rewrite Bool.andb_true_iff; split; try easy.
+    apply is_interesting_raw_renaming_extend_boring_none; easy.
+Qed.
+
+Definition is_ordered_raw_renaming_var v r :=
+  match r with
+  | raw_renaming_id => true
+  | raw_renaming_extend v' _ _ => is_less_equal_vars v v'
+  end.
+
+Fixpoint is_all_ordered_raw_renaming r :=
+  match r with
+  | raw_renaming_id => true
+  | raw_renaming_extend vl r' vr =>
+    andb
+      (is_ordered_raw_renaming_var vl r')
+      (is_all_ordered_raw_renaming r')
+  end.
+
+Lemma is_all_ordered_raw_renaming_from_extend {vl r vr} :
+  is_all_ordered_raw_renaming
+    (raw_renaming_extend vl r vr) = true ->
+  is_all_ordered_raw_renaming r = true.
+Proof.
+  destruct r; cbn;
+    try rewrite Bool.andb_true_iff; easy.
+Qed.
+
+(* TODO : move to var equations *)
+Lemma monotonic_succ_var v1 v2 :
+  is_less_equal_vars v1 v2 = true ->
+  is_less_equal_vars (succ_var v1) (succ_var v2) = true.
+Proof.
+  case_vars v1 v2; easy.
+Qed.
+
+(* TODO : move to var equations *)
+Lemma is_less_equal_shift v1 v2 v3 :
+  is_less_equal_vars v1 v2 = true ->
+  is_less_equal_vars
+    (shift_var v3 v1) (shift_var (unshift_var v1 v3) v2) = true.
+Proof.
+  case_vars v1 v3;
+    case_vars (unshift_var v1 v3) v2; try easy.
+  apply monotonic_succ_var.
+Qed.
+
+Lemma is_ordered_raw_renaming_extend_boring_some_ind r1 :
+  forall r2 vl1 vl2 vr1 vr2,
+  is_ordered_raw_renaming_var vl1 r1 = true ->
+  raw_renaming_extend_boring
+    (unshift_var vl1 vl2) r1 (unshift_var vr1 vr2) = Some r2 ->
+  is_ordered_raw_renaming_var (shift_var vl2 vl1) r2 = true.
+Proof.
+  induction r1 as [|vl3 r3 IHr vr3]; cbn;
+    intros * Heq1 Heq2.
+  - destruct var_eqb; try easy.
+    injection Heq2 as <-; easy.
+  - destruct raw_renaming_extend_boring; try easy.
+    injection Heq2 as <-; cbn.
+    apply is_less_equal_shift; easy.
+Qed.
+
+Lemma is_ordered_raw_renaming_less_equal_var v1 v2 r :
+  is_ordered_raw_renaming_var v1 r = true ->
+  is_less_equal_vars v2 v1 = true ->
+  is_ordered_raw_renaming_var v2 r = true.
+Proof.
+  destruct r; cbn; intros Heq1 Heq2; try easy.
+  apply is_less_equal_vars_transitive with (v2 := v1); easy.
+Qed.
+
+Lemma is_ordered_raw_renaming_extend_boring_some vl r vr r' :
+  is_all_ordered_raw_renaming r = true ->
+  is_ordered_raw_renaming_var vl r = true ->
+  raw_renaming_extend_boring vl r vr = Some r' ->
+  is_all_ordered_raw_renaming r' = true.
+Proof.
+  generalize dependent vl.
+  generalize dependent vr.
+  generalize dependent r'.
+  induction r as [|vl' r IHr vr']; cbn;
+    intros r' vr vl Heq1 Heq2 Heq3.
+  - destruct var_eqb; try easy.
+    injection Heq3 as <-; easy.
+  - rewrite Bool.andb_true_iff in Heq1;
+      destruct Heq1 as [Heq1 Heq4].
+    destruct raw_renaming_extend_boring eqn:Heq5; try easy.
+    injection Heq3 as <-; cbn.
+    rewrite Bool.andb_true_iff; split.
+    + apply is_ordered_raw_renaming_extend_boring_some_ind
+        with (r1 := r) (vr1 := vr') (vr2 := vr); easy.
+    + apply IHr
+        with (vl := unshift_var vl' vl) (vr := unshift_var vr' vr);
+        try easy.
+      apply is_ordered_raw_renaming_less_equal_var
+        with (v1 := vl'); try easy.
+      apply is_less_equal_vars_transitive with (v2 := vl); try easy.
+      apply is_less_equal_vars_unshift_r.
+Qed.
+
+Lemma is_all_ordered_raw_renaming_extend vl r vr :
+  is_all_ordered_raw_renaming r = true ->
+  is_ordered_raw_renaming_var vl r = true ->
+  is_all_ordered_raw_renaming
+    (interesting_raw_renaming_extend vl r vr) = true.
+Proof.
+  intros Heq1 Heq2.
+  unfold interesting_raw_renaming_extend.
+  destruct raw_renaming_extend_boring
+    eqn:Heq3; cbn; try rewrite Bool.andb_true_iff; try easy.
+  apply is_ordered_raw_renaming_extend_boring_some
+    with (vl := vl) (r := r) (vr := vr); easy.
+Qed.
+
+Definition is_normalized_raw_renaming r :=
+  andb
+    (is_all_interesting_raw_renaming r)
+    (is_all_ordered_raw_renaming r).
+
+Definition normalized_raw_renaming r :=
+  if is_normalized_raw_renaming r then sUnit else sEmpty.
+
+Lemma is_normalized_raw_renaming_from_extend {vl r vr} :
+  is_normalized_raw_renaming (raw_renaming_extend vl r vr) = true ->
+  is_normalized_raw_renaming r = true.
+Proof.
+  cbn.
+  destruct (is_normalized_raw_renaming r); try easy.
+  rewrite !Bool.andb_false_r; easy.
+Qed.
+
+Lemma normalized_raw_renaming_from_extend {vl r vr} :
+  normalized_raw_renaming (raw_renaming_extend vl r vr) ->
+  normalized_raw_renaming r.
+Proof.
+  unfold normalized_raw_renaming; cbn.
+  destruct (is_normalized_raw_renaming r); try easy.
+  rewrite !Bool.andb_false_r; easy.
+Qed.
+
+Lemma is_normalized_raw_renaming_extend_boring_none
+      r vl1 vl2 vr1 vr2 :
+  is_normalized_raw_renaming (raw_renaming_extend vl2 r vr2)
+  = true ->
+  raw_renaming_extend_boring
+    vl1 (raw_renaming_extend vl2 r vr2) vr1 = None ->
+  is_less_equal_vars vl1 vl2 = true ->
+  is_normalized_raw_renaming
+    (raw_renaming_extend vl1 (raw_renaming_extend vl2 r vr2) vr1)
+    = true.
+Proof.
+  intros Heq1 Heq2 Heq3; cbn in *.
+  rewrite Heq3, Heq1.
+  rewrite is_interesting_raw_renaming_extend_boring_none; try easy.
+  destruct (raw_renaming_extend_boring (unshift_var vl2 vl1) r
+             (unshift_var vr2 vr1)); easy.
+Qed.
+
+Lemma is_normalized_raw_renaming_extend_boring_some
+           vl r vr r' :
+  is_normalized_raw_renaming r = true ->
+  raw_renaming_extend_boring vl r vr = Some r' ->
+  is_normalized_raw_renaming r' = true.
+Proof.
+  generalize dependent vl.
+  generalize dependent vr.
+  generalize dependent r'.
+  induction r as [|vl' r IHr vr']; cbn;
+    intros r' vr vl Heq1 Heq2.
+  - destruct (var_eqb vl vr); try easy.
+    replace r' with (raw_renaming_id) by congruence.
+    easy.
+  - destruct (is_ordered_raw_renaming_var vl' r)
+      eqn:Heq4; try easy.
+    destruct (is_interesting_raw_renaming_extension vl' r vr')
+      eqn:Heq5; try easy.
+    destruct (is_normalized_raw_renaming r)
+      eqn:Heq6; try easy.
+    destruct (raw_renaming_extend_boring
+                (unshift_var vl' vl) r (unshift_var vr' vr))
+      as [r''|] eqn:Heq7; try easy.
+    replace r'
+      with (raw_renaming_extend (shift_var vl vl')
+              r'' (shift_var vr vr'))
+      by congruence; cbn.
+    replace (is_normalized_raw_renaming r'') with true
+      by (symmetry;
+          apply IHr with (vl := unshift_var vl' vl)
+            (vr := unshift_var vr' vr); easy).
+    rewrite is_ordered_raw_renaming_extend_boring_shift
+      with (r1 := r) (vr1 := vr') (vr2 := vr) by easy.
+    admit.
+Admitted.
+(*
+    rewrite (is_interesting_raw_renaming_extend_boring_shift
+               Heq5 Heq7).
+    easy.
+Qed.
+*)
+
+Lemma is_normalized_interesting_raw_renaming_extend vl r vr :
+  is_normalized_raw_renaming r = true ->
+  is_ordered_raw_renaming_var vl r = true ->
+  is_normalized_raw_renaming
+    (interesting_raw_renaming_extend vl r vr) = true.
+Proof.
+  intros Heq1 Heq2; unfold interesting_raw_renaming_extend.
+  destruct (raw_renaming_extend_boring vl r vr) as [r'|] eqn:Heq3.
+  - apply is_normalized_raw_renaming_extend_boring_some
+      with (vl := vl) (r := r) (vr := vr); easy.
+  - cbn; rewrite Heq1, Heq2.
+    rewrite is_interesting_raw_renaming_extend_boring_none by easy.
+    easy.
+Qed.
+
+Fixpoint normalized_raw_renaming_extend vl r vr :=
+  match r with
+  | raw_renaming_id => interesting_raw_renaming_extend vl r vr
+  | raw_renaming_extend vl' r' vr' =>
+    if is_less_equal_vars vl vl' then
+      interesting_raw_renaming_extend vl r vr
+    else
+      raw_renaming_extend
+        (shift_var vl vl')
+        (normalized_raw_renaming_extend
+           (unshift_var vl' vl) r' (unshift_var vr' vr))
+        (shift_var vr vr')
+  end.
+
+Set Primitive Projections.
+Record renaming :=
+  mk_renaming {
+      r_raw : raw_renaming;
+      r_normalized : normalized_raw_renaming r_raw
+    }.
+Add Printing Constructor renaming.
+Unset Primitive Projections.
+
+Definition renaming_id : renaming :=
+  mk_renaming raw_renaming_id stt.
+
+
+Lemma is_interesting_interesting_raw_renaming_extend_shift_ind
+      r1 :
+  forall r2 vl1 vl2 vl3 vl4 vr1 vr2 vr3 vr4,
+  is_interesting_raw_renaming_extension vl1 r1 vr1 = true ->
+  vl3 = unshift_var vl1 vl2 ->
+  vr3 = unshift_var vr1 vr2 ->
+  r2 = interesting_raw_renaming_extend vl3 r1 vr3 ->
+  vl4 = shift_var vl2 vl1 ->
+  vr4 = shift_var vr2 vr1 ->
+  is_interesting_raw_renaming_extension vl4 r2 vr4 = true.
+Proof.
+  intros * Heq1 -> -> -> -> ->.
+  unfold interesting_raw_renaming_extend.
+  destruct
+      (raw_renaming_extend_boring
+         (unshift_var vl1 vl2) r1
+         (unshift_var vr1 vr2))
+      as [r2|] eqn:Heq2; try easy.
+  - apply (@is_interesting_raw_renaming_extend_boring_shift r1); easy.
+  - 
+
+  induction r1 as [|vl5 r1 IHr1 vr5]; cbn;
+    unfold interesting_raw_renaming_extend;
+
+Qed.
+
+Lemma is_interesting_raw_renaming_extend_boring_shift
+      {r1 r2 vl1 vl2 vr1 vr2} :
+  is_interesting_raw_renaming_extension vl1 r1 vr1 = true ->
+  raw_renaming_extend_boring
+    (unshift_var vl1 vl2) r1 (unshift_var vr1 vr2) = Some r2 ->
+  is_interesting_raw_renaming_extension
+    (shift_var vl2 vl1) r2 (shift_var vr2 vr1) = true.
+Proof.
+  intros Heq1 Heq2.
+  apply (is_interesting_raw_renaming_extend_boring_shift_ind
+           r1 r2 vl1 vl2 _ _ vr1 vr2 _ _ Heq1 eq_refl eq_refl Heq2
+           eq_refl eq_refl).
+Qed.
+
+Lemma is_interesting_normalized_raw_renaming_extend_shift_ind
+      r1 :
+  forall vl1 vl2 vl3 vl4 vr1 vr2 vr3 vr4,
+  is_interesting_raw_renaming_extension vl1 r1 vr1 = true ->
+  vl3 = unshift_var vl1 vl2 ->
+  vr3 = unshift_var vr1 vr2 ->
+  vl4 = shift_var vl2 vl1 ->
+  vr4 = shift_var vr2 vr1 ->
+  is_interesting_raw_renaming_extension
+    vl4 (normalized_raw_renaming_extend vl3 r1 vr3) vr4 = true.
+Proof.
+  induction r1 as [|vl5 r1 IHr1 vr5];
+    cbn -[interesting_raw_renaming_extend];
+    intros * Heq1 -> -> -> ->.
   - destruct
       (raw_renaming_extend_boring
-         (unshift_var v5 (unshift_var v1 v2)) r1
-         (unshift_var_opt vo5 (unshift_var_opt vo1 vo2)))
-      as [r3|] eqn:Heq3; try easy.
-    replace r2 with
-        (raw_renaming_extend
-              (shift_var (unshift_var v1 v2) v5) r3
-              (shift_var_opt (unshift_var_opt vo1 vo2) vo5))
-      by congruence; cbn.
+        (unshift_var vl1 vl2) raw_renaming_id
+        (unshift_var vr1 vr2)) as [r2|] eqn:Heq2.
+    + apply (@is_interesting_raw_renaming_extend_boring_shift
+               raw_renaming_id); easy.
+    + cbn; rewrite transpose_pushes_squared_left,
+        transpose_pops_squared_right; easy.
+  - destruct (is_less_equal_vars (unshift_var vl1 vl2) vl5) eqn:Heq2.
+    + destruct
+        (raw_renaming_extend_boring
+          (unshift_var vl1 vl2)
+          (raw_renaming_extend vl5 r1 vr5)
+          (unshift_var vr1 vr2)) as [r2|] eqn:Heq3.
+      * apply (@is_interesting_raw_renaming_extend_boring_shift
+                 (raw_renaming_extend vl5 r1 vr5)); easy.
+      * 
+
+destruct
+      (var_eqb (unshift_var vl1 vl2) (unshift_var vr1 vr2))
+      eqn:Heq3; cbn;
+      rewrite Bool.negb_true_iff, var_eqb_false, ?var_eqb_true in *.
+    + apply shift_neq; easy.
+    + 
+  - 
+    + destruct
+        (raw_renaming_extend_boring
+           (unshift_var vl5 (unshift_var vl1 vl2)) r1
+           (unshift_var vr5 (unshift_var vr1 vr2)))
+        as [r2|] eqn:Heq3.
+      * admit.
+      * 
+
     eapply IHr1
-      with (v1 := unshift_var v5 v1)
-           (vo1 := unshift_var_opt vo5 vo1)
-           (v2 := unshift_var (shift_var v1 v5) v2)
-           (vo2 := unshift_var_opt (shift_var_opt vo1 vo5) vo2)
-           (v3 := unshift_var v5 (unshift_var v1 v2))
-           (vo3 := unshift_var_opt vo5 (unshift_var_opt vo1 vo2));
+      with (vl1 := unshift_var vl5 vl1)
+           (vr1 := unshift_var vr5 vr1)
+           (vl2 := unshift_var (shift_var vl1 vl5) vl2)
+           (vr2 := unshift_var (shift_var vr1 vr5) vr2)
+           (vl3 := unshift_var vl5 (unshift_var vl1 vl2))
+           (vr3 := unshift_var vr5 (unshift_var vr1 vr2));
       try easy.
     + rewrite transpose_pops_reverse_right; easy.
     + rewrite transpose_pushes_reverse_left; easy.
     + rewrite transpose_pops_reverse_middle; easy.
     + rewrite transpose_pushes_reverse_middle; easy.
-Qed.
 
-Lemma is_interesting_raw_renaming_extend_boring_shift
-      {r1 r2 v1 v2 vo1 vo2} :
-  is_interesting_raw_renaming_extension v1 r1 vo1 = true ->
-  raw_renaming_extend_boring
-    (unshift_var v1 v2) r1 (unshift_var_opt vo1 vo2) = Some r2 ->
-  is_interesting_raw_renaming_extension
-    (shift_var v2 v1) r2 (shift_var_opt vo2 vo1) = true.
-Proof.
-  intros Heq1 Heq2.
-  apply (is_interesting_raw_renaming_extend_boring_shift_ind
-           r1 r2 v1 v2 _ _ vo1 vo2 _ _ Heq1 eq_refl eq_refl Heq2
-           eq_refl eq_refl).
-Qed.
+  - 
 
-Lemma is_ordered_raw_renaming_extend_boring_shift
-           r1 r2 v1 v2 vo1 vo2 :
-  is_ordered_raw_renaming_var v1 r1 = true ->
-  raw_renaming_extend_boring
-    (unshift_var v1 v2) r1 (unshift_var_opt vo1 vo2)
-  = Some r2 ->
-  is_ordered_raw_renaming_var (shift_var v2 v1) r2 = true.
-Proof.
-  generalize dependent v1.
-  generalize dependent v2.
-  generalize dependent vo1.
-  generalize dependent vo2.
-  generalize dependent r2.
-  induction r1 as [|v3 r3 IHr vo3]; cbn;
-    intros r2 vo2 vo1 v2 v1 Heq1 Heq2.
-  - destruct var_opt_var_eqb; try easy.
-    replace r2 with raw_renaming_id by congruence; easy.
-  - destruct
-      (raw_renaming_extend_boring
-         (unshift_var v3 (unshift_var v1 v2)) r3
-         (unshift_var_opt vo3 (unshift_var_opt vo1 vo2)));
-      try easy.
-    replace r2
-      with (raw_renaming_extend
-              (shift_var (unshift_var v1 v2) v3) r
-              (shift_var_opt (unshift_var_opt vo1 vo2) vo3))
-      by congruence; cbn.
-    generalize Heq1.
-    case_vars v1 v2; case_vars v1 v3; try easy.
-    + case_vars (pred_var v2) v3; easy.
-    + case_vars (pred_var v2) v1; easy.
-Qed.
-
-Lemma is_normalized_raw_renaming_extend_boring_some
-           v r vo r' :
-  is_normalized_raw_renaming r = true ->
-  raw_renaming_extend_boring v r vo = Some r' ->
-  is_normalized_raw_renaming r' = true.
-Proof.
-  generalize dependent v.
-  generalize dependent vo.
-  generalize dependent r'.
-  induction r as [|v' r IHr vo']; cbn;
-    intros r' vo v Heq1 Heq2.
-  - destruct (var_opt_var_eqb vo v); try easy.
-    replace r' with (raw_renaming_id) by congruence.
-    easy.
-  - destruct (is_ordered_raw_renaming_var v' r)
-      eqn:Heq4; try easy.
-    destruct (is_interesting_raw_renaming_extension v' r vo')
-      eqn:Heq5; try easy.
-    destruct (is_normalized_raw_renaming r)
-      eqn:Heq6; try easy.
-    destruct (raw_renaming_extend_boring
-                (unshift_var v' v) r (unshift_var_opt vo' vo))
-      as [r''|] eqn:Heq7; try easy.
-    replace r'
-      with (raw_renaming_extend (shift_var v v')
-              r'' (shift_var_opt vo vo'))
-      by congruence; cbn.
-    replace (is_normalized_raw_renaming r'') with true
-      by (symmetry;
-          apply IHr with (v := unshift_var v' v)
-            (vo := unshift_var_opt vo' vo); easy).
-    rewrite is_ordered_raw_renaming_extend_boring_shift
-      with (r1 := r) (vo1 := vo') (vo2 := vo) by easy.
-    rewrite (is_interesting_raw_renaming_extend_boring_shift
-               Heq5 Heq7).
-    easy.
-Qed.
-
-Fixpoint normalized_raw_renaming_extend v r vo :=
-  match r with
-  | raw_renaming_id =>
-    match raw_renaming_extend_boring v r vo with
-    | Some r => r
-    | None => raw_renaming_extend v r vo
-    end
-  | raw_renaming_extend v' r' vo' =>
-    if is_less_equal_vars v v' then
-      match raw_renaming_extend_boring v r vo with
-      | Some r => r
-      | None => raw_renaming_extend v r vo
-      end
-    else
-      raw_renaming_extend
-        (shift_var v v')
-        (normalized_raw_renaming_extend
-           (unshift_var v' v) r' (unshift_var_opt vo' vo))
-        (shift_var_opt vo vo')
-  end.
-
-Lemma normalized_raw_renaming_extend_normalized v r vo :
+Lemma normalized_raw_renaming_extend_normalized vl r vr :
   normalized_raw_renaming r ->
   normalized_raw_renaming
-    (normalized_raw_renaming_extend v r vo).
+    (normalized_raw_renaming_extend vl r vr).
 Proof.
   unfold normalized_raw_renaming.
   destruct (is_normalized_raw_renaming r) eqn:Heq1;
     try easy; intros _.
-  generalize dependent v.
-  generalize dependent vo.
-  induction r as [|v' r IHr vo']; intros vo v.
-  - cbn; destruct var_opt_var_eqb eqn:Heq2; cbn; try easy.
+  generalize dependent vl.
+  generalize dependent vr.
+  induction r as [|vl' r IHr vr']; intros vr vl.
+  - cbn; destruct var_eqb eqn:Heq2; cbn; try easy.
     rewrite Heq2; easy.
   - unfold normalized_raw_renaming_extend.
-    destruct (is_less_equal_vars v v') eqn:Heq6.
+    fold normalized_raw_renaming_extend.
+    destruct (is_less_equal_vars vl vl') eqn:Heq6.
     + destruct (raw_renaming_extend_boring
-                  v (raw_renaming_extend v' r vo') vo)
+                  vl (raw_renaming_extend vl' r vr') vr)
                eqn:Heq7.
       * rewrite is_normalized_raw_renaming_extend_boring_some
-          with (r := raw_renaming_extend v' r vo')
-               (v := v) (vo := vo); easy.
+          with (r := raw_renaming_extend vl' r vr')
+               (vl := vl) (vr := vr); easy.
       * rewrite is_normalized_raw_renaming_extend_boring_none
-          with (r := r) (v1 := v) (v2 := v')
-               (vo1 := vo) (vo2 := vo'); try easy.
-    + specialize
-        (IHr eq_refl (unshift_var_opt vo' vo) (unshift_var v' v)).
+          with (r := r) (vl1 := vl) (vl2 := vl')
+               (vr1 := vr) (vr2 := vr'); try easy.
+    + apply is_normalized_raw_renaming_from_extend in Heq1 as Heq2.
+      specialize
+        (IHr Heq2 (unshift_var vr' vr) (unshift_var vl' vl)).
       destruct (is_normalized_raw_renaming
                   (normalized_raw_renaming_extend
-                     (unshift_var v' v) r (unshift_var_opt vo' vo)))
+                     (unshift_var vl' vl) r (unshift_var vr' vr)))
                eqn:Heq7; try easy.
 Qed.
 
