src/VarEquations.v
@@ -157,85 +157,43 @@ Proof.
   - destruct (le_gt_dec l2 l1); cbn; try easy; lia.
 Qed.
 
-Lemma reduce_pop_var_bound_zero v1 v2 :
-  v_label_opt v2 = None ->
-  v_nat v2 = 0 ->
-  pop_var v1 v2 = v1.
-Proof. destruct v1 as [n1|l1], v2 as [n2|[|l2]]; easy. Qed.
+Lemma reduce_pop_var_none v1 :
+  pop_var v1 None = v1.
+Proof. easy. Qed.
 
-Lemma reduce_pop_var_free v1 v2 :
-  v_label_opt v2 <> None ->
-  pop_var v1 v2 = shift_var v1 v2.
-Proof. destruct v1 as [n1|l1], v2 as [n2|l2]; easy. Qed.
+Lemma reduce_pop_var_some v1 v2 :
+  pop_var v1 (Some v2) = shift_var v1 v2.
+Proof. easy. Qed.
 
-Lemma reduce_pop_var_bound_nonzero v1 v2 :
-  v_label_opt v2 = None ->
-  v_nat v2 <> 0 ->
-  pop_var v1 v2 = shift_var v1 (pred_var v2).
-Proof.
-  destruct v1 as [n1|l1], v2 as [n2|[|l2]]; easy.
-Qed.
-
-Lemma reduce_push_var_none v :
-  push_var None v = shift_var zero_var v.
-Proof. destruct v as [n|l]; easy. Qed.
-
-Lemma reduce_push_var_some_eq v1 v2 :
+Lemma reduce_push_var_eq v1 v2 :
   v_label_opt v1 = v_label_opt v2 ->
   v_nat v1 = v_nat v2 ->
-  push_var (Some v1) v2 = zero_var.
+  push_var v1 v2 = None.
 Proof.
   intros Heq1 Heq2; rewrite (lift_var_eq Heq1 Heq2).
-  unfold push_var, var_opt_var_eqb.
-  destruct (var_opt_var_dec (Some v2) v2); easy.
+  unfold push_var, var_eqb.
+  destruct (var_dec v2 v2); easy.
 Qed.
 
-Lemma reduce_push_var_some_distinct v1 v2 :
+Lemma reduce_push_var_distinct v1 v2 :
   v_label_opt v1 <> v_label_opt v2 ->
-  push_var (Some v1) v2 = shift_var zero_var v2.
+  push_var v1 v2 = Some v2.
 Proof.
   intros.
-  rewrite <- reduce_unshift_var_distinct
-    with (v1 := v1) (v2 := shift_var zero_var v2)
-    by (reduce_vars_beta; easy).
-  unfold push_var, var_opt_var_eqb.
-  destruct (var_opt_var_dec (Some v1) v2);
-    try congruence; easy.
+  unfold push_var, var_eqb.
+  destruct (var_dec v1 v2); try congruence.
+  rewrite reduce_unshift_var_distinct; easy.
 Qed.
 
-Lemma reduce_push_var_some_neq v1 v2 :
+Lemma reduce_push_var_neq v1 v2 :
   v_label_opt v1 = v_label_opt v2 ->
   v_nat v1 <> v_nat v2 ->
-  push_var (Some v1) v2
-  = unshift_var v1 (shift_var zero_var v2).
+  push_var v1 v2 = Some (unshift_var v1 v2).
 Proof.
-  intros; unfold push_var, var_opt_var_eqb.
-  destruct (var_opt_var_dec (Some v1) v2);
+  intros; unfold push_var, var_eqb.
+  destruct (var_dec v1 v2);
     try congruence; easy.
 Qed.
-
-Lemma reduce_swap_var_free v :
-  v_label_opt v <> None ->
-  swap_var v = v.
-Proof. destruct v as [n|l]; easy. Qed.
-
-Lemma reduce_swap_var_bound_zero v :
-  v_label_opt v = None ->
-  v_nat v = 0 ->
-  swap_var v = succ_var zero_var.
-Proof. destruct v as [n|[|l]]; easy. Qed.
-
-Lemma reduce_swap_var_bound_one v :
-  v_label_opt v = None ->
-  v_nat v = 1 ->
-  swap_var v = zero_var.
-Proof. destruct v as [n|[|[|l]]]; easy. Qed.
-
-Lemma reduce_swap_var_bound_gt_one v :
-  v_label_opt v = None ->
-  v_nat v > 1 ->
-  swap_var v = v.
-Proof. destruct v as [n|[|[|l]]]; cbn; try easy; lia. Qed.
 
 Lemma reduce_pred_var_succ_var v :
   pred_var (succ_var v) = v.
@@ -251,24 +209,6 @@ Proof.
   intros; unfold pred_var, succ_var.
   apply lift_var_eq; reduce_vars_beta; try easy; lia.
 Qed.
-
-Lemma reduce_lift_var_op_bound_zero op v :
-  v_label_opt v = None ->
-  v_nat v = 0 ->
-  lift_var_op op v = v.
-Proof. destruct v as [n|l]; cbn; intros; subst; easy. Qed.
-
-Lemma reduce_lift_var_op_free op v :
-  v_label_opt v <> None ->
-  lift_var_op op v = shift_var zero_var (op v).
-Proof. destruct v as [n|l]; easy. Qed.
-
-Lemma reduce_lift_var_op_bound_nonzero op v :
-  v_label_opt v = None ->
-  v_nat v <> 0 ->
-  lift_var_op op v
-  = shift_var zero_var (op (unshift_var zero_var v)).
-Proof. destruct v as [n|[|l]]; easy. Qed.
 
 Lemma reduce_is_less_equal_var_distinct v1 v2 :
   v_label_opt v1 <> v_label_opt v2 ->
@@ -315,30 +255,25 @@ Hint Rewrite reduce_v_label_opt_beta reduce_v_nat_beta
      reduce_v_label_opt_succ_beta reduce_v_nat_succ_beta
      reduce_v_label_opt_pred_beta reduce_v_nat_pred_beta
      reduce_v_label_opt_shift_beta reduce_v_label_opt_unshift_beta
-     reduce_push_var_none reduce_pred_var_succ_var
+     reduce_pred_var_succ_var reduce_pop_var_none reduce_pop_var_some
   : reduce_vars.
 
 Hint Rewrite reduce_shift_var_distinct
-     reduce_unshift_var_distinct reduce_pop_var_free
-     reduce_push_var_some_distinct reduce_swap_var_free
-     reduce_lift_var_op_free
+     reduce_unshift_var_distinct
+     reduce_push_var_distinct
      reduce_is_less_equal_var_distinct
      using solve_v_label_opt_equation : reduce_vars.
 
 Hint Rewrite reduce_shift_var_ge reduce_shift_var_lt
      reduce_unshift_var_le reduce_unshift_var_gt
-     reduce_pop_var_bound_zero reduce_pop_var_bound_nonzero
-     reduce_push_var_some_eq reduce_push_var_some_neq
-     reduce_swap_var_bound_zero reduce_swap_var_bound_one
-     reduce_swap_var_bound_gt_one reduce_succ_var_pred_var
-     reduce_lift_var_op_bound_zero
-     reduce_lift_var_op_bound_nonzero
+     reduce_push_var_eq reduce_push_var_neq
+     reduce_succ_var_pred_var
      reduce_is_less_equal_var_ge reduce_is_less_equal_var_lt
      using solve_v_label_opt_and_v_nat_equation : reduce_vars.
 
 Ltac reduce_vars :=
   try repeat
-      (autorewrite with reduce_vars; cbn);
+      (autorewrite with reduce_vars in *; cbn in *);
   try repeat
     ((rewrite_strat (bottomup (hints reduce_vars))); cbn).
 
@@ -383,38 +318,40 @@ Ltac case_vars v1 v2 :=
     try rewrite (eta_reduce_var v2);
     try solve [exfalso; try congruence; try lia].
 
-Ltac case_var_zero v :=
-  case_vars zero_var v.
+Tactic Notation "case_var_var_opt" constr(v1) constr(vo2) "as" simple_intropattern(v2) :=
+  destruct vo2 as [v2|];
+    [case_vars v1 v2 |reduce_vars].
 
-Ltac case_var_one v :=
-  case_vars (succ_var zero_var) v.
+Tactic Notation "case_var_var_opt" constr(v1) constr(vo2) :=
+  let v2 := fresh "v" in
+  case_var_var_opt v1 vo2 as v2.
+
+Tactic Notation "case_var_opt" constr(vo)
+       "as" simple_intropattern(v) :=
+  destruct vo as [v|]; reduce_vars.
+
+Tactic Notation "case_var_opt" constr(vo) :=
+  let v := fresh "v" in
+  case_var_opt vo as v.
+
+Tactic Notation "case_var_opt_opt" constr(vo) "as" simple_intropattern(v) :=
+  destruct vo as [[v|]|]; reduce_vars.
+
+Tactic Notation "case_var_opt_opt" constr(vo) :=
+  let v := fresh "v" in
+  case_var_opt_opt vo as v.
 
 (* Identities *)
 
-Lemma pop_zero_identity :
-  pop_var zero_var =v= 1.
-Proof.
-  intros v.
-  case_var_zero v; easy.
-Qed.
-
-Lemma push_zero_identity :
-  push_var (Some zero_var) =v= 1.
-Proof.
-  intros v.
-  case_var_zero v; easy.
-Qed.
-
 Lemma pop_push_identity v :
-  pop_var v @ push_var (Some v) =v= 1.
+  pop_var v @ push_var v =v= 1.
 Proof.
   intros v'.
-  case_vars v v'; try easy;
-    case_var_zero v'; easy.
+  case_vars v v'; easy.
 Qed.
 
-Lemma pop_push_identity' v op :
-  pop_var v @ (push_var (Some v) @ op) =v= op.
+Lemma pop_push_identity' {N} v (op : var_op N 0) :
+  pop_var v @ (push_var v @ op) =v= op.
 Proof.
   rewrite var_op_associative, pop_push_identity,
     var_op_left_identity.
@@ -422,15 +359,14 @@ Proof.
 Qed.
 
 Lemma push_pop_identity v :
-  push_var (Some v) @ pop_var v =v= 1.
+  push_var v @ pop_var v =v= 1.
 Proof.
   intros v'.
-  case_var_zero v'; try easy;
-    case_vars v v'; easy.
+  case_var_var_opt v v'; easy.
 Qed.
 
-Lemma push_pop_identity' v op :
-  push_var (Some v) @ (pop_var v @ op) =v= op.
+Lemma push_pop_identity' {N} v (op : var_op N 1) :
+  push_var v @ (pop_var v @ op) =v= op.
 Proof.
   rewrite var_op_associative,
     push_pop_identity, var_op_left_identity.
@@ -441,11 +377,10 @@ Lemma swap_swap_identity :
   swap_var @ swap_var =v= 1.
 Proof.
   intros v.
-  case_var_zero v; try easy.
-  case_var_one v; easy.
+  case_var_opt_opt v; easy.
 Qed.
 
-Lemma swap_swap_identity' op :
+Lemma swap_swap_identity' {N} (op : var_op N 2) :
   swap_var @ (swap_var @ op) =v= op.
 Proof.
   rewrite var_op_associative,
@@ -455,28 +390,27 @@ Qed.
 
 (* [lift_var_op] distributes over composition and identity *)
 
-Lemma lift_var_op_compose op1 op2 :
+Lemma lift_var_op_compose
+      {N M O} (op1 : var_op M O) (op2 : var_op N M) :
   lift_var_op (op1 @ op2)
   =v= lift_var_op op1 @ lift_var_op op2.
 Proof.
-  intros v.
-  case_var_zero v; try easy.
-  - case_var_zero (op2 (pred_var v)); easy.
-  - case_var_zero (op2 v); easy.
+  intros vo.
+  case_var_opt vo; easy.
 Qed.
 
-Lemma lift_var_op_id :
-  lift_var_op 1 =v= 1.
+Lemma lift_var_op_id {N} :
+  @lift_var_op N N 1 =v= 1.
 Proof.
-  intros v.
-  case_var_zero v; easy.
+  intros vo.
+  case_var_opt vo; easy.
 Qed.
 
 (* Tactic to simplify compositions of var operations *)
 
-Hint Rewrite <- var_op_associative
+Hint Rewrite <- @var_op_associative
   : normalize_var_op_compose.
-Hint Rewrite var_op_left_identity var_op_right_identity
+Hint Rewrite @var_op_left_identity @var_op_right_identity
   : normalize_var_op_compose.
 
 Hint Rewrite @lift_var_op_id @lift_var_op_compose
@@ -492,14 +426,11 @@ Lemma transpose_swap_lifted op :
   swap_var @ lift_var_op (lift_var_op op)
   =v= lift_var_op (lift_var_op op) @ swap_var.
 Proof.
-  intros v.
-  case_var_zero v; try easy.
-  - case_var_one v; try easy.
-    case_var_zero (op (pred_var (pred_var v))); easy.
-  - case_var_zero (op v); easy.
+  intros vo.
+  case_var_opt_opt vo; easy.
 Qed.
 
-Lemma transpose_swap_lifted' op1 op2 :
+Lemma transpose_swap_lifted' op1 {N} (op2 : var_op N 2) :
   swap_var @ (lift_var_op (lift_var_op op1) @ op2)
   =v= lift_var_op (lift_var_op op1) @ (swap_var @ op2).
 Proof.
@@ -529,25 +460,14 @@ Lemma transpose_pops v1 v2 :
       @ lift_var_op (pop_var (unshift_var v2 v1))
       @ swap_var.
 Proof.
-  intros v3.
-  case_var_zero v3; case_var_one v3.
-  - case_vars v1 v2.
-    + case_vars (pred_var (pred_var v3)) v1; try easy.
-      case_vars (pred_var (pred_var v3)) v2; easy.
-    + case_vars (pred_var (pred_var v3)) v1; easy.
-    + case_vars (pred_var v3) v1; try easy.
-      case_vars (pred_var (pred_var v3)) v2; try easy.
-    + case_vars (pred_var (pred_var v3)) v1; easy.
-  - case_var_zero v2; easy.
-  - case_vars v1 v2; case_var_zero v1; easy.
-  - case_vars v2 v1;
-      case_vars v3 v2; try easy.
-    + case_vars v3 (pred_var v1); easy.
-    + case_vars v3 (pred_var v1); easy.
-    + case_vars v1 v3; easy.
+  intros vo3.
+  case_var_opt_opt vo3 as v3; try easy;
+    case_vars v1 v2; try easy;
+      case_vars (unshift_var v2 v1) v3; try easy;
+        case_vars v3 v2; easy.
 Qed.
 
-Lemma transpose_pops' v1 v2 op :
+Lemma transpose_pops' v1 v2 {N} (op : var_op N 2) :
   pop_var v1 @ lift_var_op (pop_var v2) @ op
   =v= pop_var (shift_var v1 v2)
       @ lift_var_op (pop_var (unshift_var v2 v1))
@@ -604,10 +524,9 @@ Lemma transpose_pops_reverse_left v1 v2 v3 :
     (shift_var (unshift_var v2 v1) v3)
   = shift_var v1 (shift_var v2 v3).
 Proof.
-  case_vars v2 v1; case_vars v3 v2; try easy.
-  - case_vars (pred_var v1) v3; easy.
-  - case_vars (pred_var v1) v3; easy.
-  - case_vars v1 v3; easy.
+  case_vars v2 v1;
+    case_vars (unshift_var v2 v1) v3; try easy;
+      case_vars v3 v2; easy.
 Qed.
 
 Lemma transpose_pops_reverse_middle v1 v2 v3 :
@@ -618,10 +537,9 @@ Lemma transpose_pops_reverse_middle v1 v2 v3 :
       (shift_var (unshift_var v2 v1) v3)
       (shift_var v1 v2).
 Proof.
-  case_vars v2 v1; case_vars v3 v2; try easy.
-  - case_vars (pred_var v1) v3; easy.
-  - case_vars (pred_var v1) v3; easy.
-  - case_vars v1 v3; easy.
+  case_vars v2 v1;
+    case_vars (unshift_var v2 v1) v3; try easy;
+      case_vars v3 v2; easy.
 Qed.
 
 Lemma transpose_pops_reverse_right v1 v2 v3 :
@@ -631,10 +549,9 @@ Lemma transpose_pops_reverse_right v1 v2 v3 :
   = unshift_var v3
       (unshift_var v2 v1).
 Proof.
-  case_vars v2 v1; case_vars v3 v2; try easy.
-  - case_vars (pred_var v1) v3; easy.
-  - case_vars (pred_var v1) v3; easy.
-  - case_vars v1 v3; easy.
+  case_vars v2 v1;
+    case_vars (unshift_var v2 v1) v3; try easy;
+      case_vars v3 v2; easy.
 Qed.
 
 (* Permutations of "push" operations. As with the pop
@@ -644,27 +561,23 @@ Qed.
    equations on those transpositions required to define the
    full group of permutations. *)
 
-Lemma transpose_pushes vo1 vo2 :
-  lift_var_op (push_var vo1) @ push_var vo2
+Lemma transpose_pushes v1 v2 :
+  lift_var_op (push_var v1) @ push_var v2
   =v= swap_var
-      @ lift_var_op (push_var (unshift_var_opt vo1 vo2))
-      @ push_var (shift_var_opt vo2 vo1).
+      @ lift_var_op (push_var (unshift_var v1 v2))
+      @ push_var (shift_var v2 v1).
 Proof.
   intros v3.
-  destruct vo1 as [v1|], vo2 as [v2|]; simplify_var_ops; cbn.
-  - case_var_zero v3; case_vars v1 v2; case_vars v3 v1; try easy;
-      case_vars v3 v2; try easy;
-        case_vars (pred_var v3) v1; easy.
-  - case_var_zero v3; case_vars v1 v3; easy.
-  - case_var_zero v3; case_vars v2 v3; easy.
-  - case_var_zero v3; easy.
+  case_vars v1 v2;
+    case_vars (shift_var v2 v1) v3; try easy;
+      case_vars v2 v3; easy.
 Qed.
 
-Lemma transpose_pushes' vo1 vo2 op :
-  lift_var_op (push_var vo1) @ push_var vo2 @ op
+Lemma transpose_pushes' v1 v2 {N} (op : var_op N 0) :
+  lift_var_op (push_var v1) @ push_var v2 @ op
   =v= swap_var
-      @ lift_var_op (push_var (unshift_var_opt vo1 vo2))
-      @ push_var (shift_var_opt vo2 vo1)
+      @ lift_var_op (push_var (unshift_var v1 v2))
+      @ push_var (shift_var v2 v1)
       @ op.
 Proof.
   rewrite var_op_associative.
@@ -673,57 +586,44 @@ Proof.
   easy.
 Qed.
 
-
-Lemma transpose_pushes_squared_left vo1 vo2 :
-  unshift_var_opt
-    (unshift_var_opt vo1 vo2) (shift_var_opt vo2 vo1)
-  = vo1.
+Lemma transpose_pushes_squared_left v1 v2 :
+  unshift_var (unshift_var v1 v2) (shift_var v2 v1) = v1.
 Proof.
-  destruct vo1 as [v1|], vo2 as [v2|]; cbn; try easy.
-  rewrite transpose_pops_squared_right; easy.
+  apply transpose_pops_squared_right.
 Qed.
 
-Lemma transpose_pushes_squared_right vo1 vo2 :
-  shift_var_opt
-    (shift_var_opt vo2 vo1) (unshift_var_opt vo1 vo2)
-  = vo2.
+Lemma transpose_pushes_squared_right v1 v2 :
+  shift_var (shift_var v2 v1) (unshift_var v1 v2) = v2.
 Proof.
-  destruct vo1 as [v1|], vo2 as [v2|]; cbn; try easy.
-  rewrite transpose_pops_squared_left; easy.
+  apply transpose_pops_squared_left.
 Qed.
 
-Lemma transpose_pushes_reverse_left vo1 vo2 vo3 :
-  unshift_var_opt (unshift_var_opt vo1 vo2)
-    (unshift_var_opt (shift_var_opt vo2 vo1) vo3)
-  = unshift_var_opt vo1 (unshift_var_opt vo2 vo3).
+Lemma transpose_pushes_reverse_left v1 v2 v3 :
+  unshift_var (unshift_var v1 v2)
+    (unshift_var (shift_var v2 v1) v3)
+  = unshift_var v1 (unshift_var v2 v3).
 Proof.
-  destruct vo1 as [v1|], vo2 as [v2|], vo3 as [v3|];
-    cbn in *; try easy.
-  rewrite transpose_pops_reverse_right; easy.
+  apply transpose_pops_reverse_right.
 Qed.
 
-Lemma transpose_pushes_reverse_middle vo1 vo2 vo3 :
-  unshift_var_opt
-    (shift_var_opt (unshift_var_opt vo2 vo3) vo1)
-    (shift_var_opt vo3 vo2)
-  = shift_var_opt
-      (unshift_var_opt (shift_var_opt vo2 vo1) vo3)
-      (unshift_var_opt vo1 vo2).
+Lemma transpose_pushes_reverse_middle v1 v2 v3 :
+  unshift_var
+    (shift_var (unshift_var v2 v3) v1)
+    (shift_var v3 v2)
+  = shift_var
+      (unshift_var (shift_var v2 v1) v3)
+      (unshift_var v1 v2).
 Proof.
-  destruct vo1 as [v1|], vo2 as [v2|], vo3 as [v3|];
-    cbn in *; try easy.
   rewrite transpose_pops_reverse_middle; easy.
 Qed.
 
-Lemma transpose_pushes_reverse_right vo1 vo2 vo3 :
-  shift_var_opt
-    (shift_var_opt vo3 vo2)
-    (shift_var_opt (unshift_var_opt vo2 vo3) vo1)
-  = shift_var_opt vo3 (shift_var_opt vo2 vo1).
+Lemma transpose_pushes_reverse_right v1 v2 v3 :
+  shift_var
+    (shift_var v3 v2)
+    (shift_var (unshift_var v2 v3) v1)
+  = shift_var v3 (shift_var v2 v1).
 Proof.
-  destruct vo1 as [v1|], vo2 as [v2|], vo3 as [v3|];
-    cbn in *; try easy.
-  rewrite transpose_pops_reverse_left; easy.
+  apply transpose_pops_reverse_left.
 Qed.
 
 (* Moving pushes in front of pops.
@@ -738,39 +638,25 @@ Qed.
    permutations, but some of the "reverse" equations are
    still relevant.  *)
 
-Lemma transpose_push_pop vo1 v2 :
-  vo1 <> Some v2 ->
-  push_var vo1 @ pop_var v2
-  =v= lift_var_op (pop_var (unshift_var_opt_var vo1 v2))
+Lemma transpose_push_pop v1 v2 :
+  v1 <> v2 ->
+  push_var v1 @ pop_var v2
+  =v= lift_var_op (pop_var (unshift_var v1 v2))
       @ swap_var
-      @ lift_var_op (push_var (unshift_var_var_opt v2 vo1)).
+      @ lift_var_op (push_var (unshift_var v2 v1)).
 Proof.
-  intros Hirr v3.
-  destruct vo1 as [v1|]; simplify_var_ops; cbn.
-  - assert (v1 <> v2) by congruence.
-    case_var_zero v3; case_vars v1 v2.
-    + case_vars (pred_var v3) v1; try easy.
-      case_vars (pred_var v3) v2; easy.
-    + case_vars v3 v1; try easy.
-      case_vars (pred_var v3) v2; easy.
-    + case_vars (pred_var v3) v1; easy.
-    + case_vars v3 v2; easy.
-    + case_vars v3 v2; easy.
-    + case_vars v3 v2; easy.
-    + case_vars v3 v1; try easy.
-      case_vars v3 v2; easy.
-    + case_vars (pred_var v1) v3; try easy.
-      case_vars v3 v2; easy.
-    + case_vars v3 v1; easy.
-  - case_var_zero v3; easy.
+  intros Hirr vo3.
+  case_vars v1 v2;
+    case_var_var_opt (unshift_var v2 v1) vo3 as v3; try easy;
+      case_vars v2 v3; easy.
 Qed.
 
-Lemma transpose_push_pop' vo1 v2 op :
-  vo1 <> Some v2 ->
-  push_var vo1 @ pop_var v2 @ op
-  =v= lift_var_op (pop_var (unshift_var_opt_var vo1 v2))
+Lemma transpose_push_pop' v1 v2 {N} (op : var_op N 1) :
+  v1 <> v2 ->
+  push_var v1 @ pop_var v2 @ op
+  =v= lift_var_op (pop_var (unshift_var v1 v2))
       @ swap_var
-      @ lift_var_op (push_var (unshift_var_var_opt v2 vo1))
+      @ lift_var_op (push_var (unshift_var v2 v1))
       @ op.
 Proof.
   intros Hneq.
@@ -780,17 +666,15 @@ Proof.
   easy.
 Qed.
 
-Lemma transpose_push_push_pop_reverse_left vo1 vo2 v3 :
-  unshift_var_opt_var
-    (unshift_var_opt vo1 vo2)
-    (unshift_var_opt_var (shift_var_opt vo2 vo1) v3)
-  = unshift_var_opt_var vo1 (unshift_var_opt_var vo2 v3).
+Lemma transpose_push_push_pop_reverse_left v1 v2 v3 :
+  unshift_var
+    (unshift_var v1 v2) (unshift_var (shift_var v2 v1) v3)
+  = unshift_var v1 (unshift_var v2 v3).
 Proof.
-  destruct vo1 as [v1|], vo2 as [v2|]; cbn; try easy.
-  rewrite transpose_pops_reverse_right; easy.
+  apply transpose_pops_reverse_right.
 Qed.
 
-Lemma transpose_push_push_pop_reverse_middle_aux v1 v2 v3 :
+Lemma transpose_push_push_pop_reverse_middle v1 v2 v3 :
   unshift_var
     (unshift_var (unshift_var v2 v3) v1)
     (unshift_var v3 v2)
@@ -798,82 +682,48 @@ Lemma transpose_push_push_pop_reverse_middle_aux v1 v2 v3 :
       (unshift_var (shift_var v2 v1) v3)
       (unshift_var v1 v2).
 Proof.
-  case_vars v2 v1; case_vars v3 v2; try easy.
-  - case_vars (pred_var v3) v1; easy.
-  - case_vars (pred_var v3) v1; easy.
-  - case_vars v1 v3; easy.
+  case_vars v1 v2;
+    case_vars (shift_var v2 v1) v3; try easy;
+      case_vars v2 v3; easy.
 Qed.
 
-Lemma transpose_push_push_pop_reverse_middle vo1 vo2 v3 :
-  unshift_var_opt
-    (unshift_var_var_opt
-       (unshift_var_opt_var vo2 v3) vo1)
-    (unshift_var_var_opt v3 vo2)
-  = unshift_var_var_opt
-      (unshift_var_opt_var (shift_var_opt vo2 vo1) v3)
-      (unshift_var_opt vo1 vo2).
-Proof.
-  destruct vo1 as [v1|], vo2 as [v2|]; cbn; try easy.
-  rewrite transpose_push_push_pop_reverse_middle_aux; easy.
-Qed.
-
-Lemma transpose_push_push_pop_reverse_right_aux v1 v2 v3 :
+Lemma transpose_push_push_pop_reverse_right v1 v2 v3 :
   v1 <> unshift_var v2 v3 ->
   shift_var
     (unshift_var v3 v2)
       (unshift_var (unshift_var v2 v3) v1)
   = unshift_var v3 (shift_var v2 v1).
 Proof.
-  case_vars v2 v1; case_vars v3 v2; try easy.
-  - case_vars (pred_var v3) v1; easy.
-  - case_vars v1 v3; easy.
+  case_vars v1 v2;
+    case_vars (shift_var v2 v1) v3; try easy;
+      case_vars v2 v3; easy.
 Qed.
 
-Lemma transpose_push_push_pop_reverse_right vo1 vo2 v3 :
-  vo1 <> Some (unshift_var_opt_var vo2 v3) ->
-  shift_var_opt
-    (unshift_var_var_opt v3 vo2)
-      (unshift_var_var_opt (unshift_var_opt_var vo2 v3) vo1)
-  = unshift_var_var_opt v3 (shift_var_opt vo2 vo1).
-Proof.
-  destruct vo1 as [v1|], vo2 as [v2|];
-    cbn; try easy; intros.
-  rewrite transpose_push_push_pop_reverse_right_aux; try easy;
-    congruence.
-Qed.
-
-Lemma transpose_push_pop_pop_reverse_left vo1 v2 v3 :
-  (unshift_var_var_opt v2 vo1) <> Some v3 ->
+Lemma transpose_push_pop_pop_reverse_left v1 v2 v3 :
+  v3 <> unshift_var v2 v1 ->
   shift_var
-    (unshift_var_opt_var vo1 v2)
-    (unshift_var_opt_var (unshift_var_var_opt v2 vo1) v3)
-  = unshift_var_opt_var vo1 (shift_var v2 v3).
+    (unshift_var v1 v2) (unshift_var (unshift_var v2 v1) v3)
+  = unshift_var v1 (shift_var v2 v3).
 Proof.
-  destruct vo1 as [v1|]; cbn; try easy; intros.
-  rewrite transpose_push_push_pop_reverse_right_aux; try easy;
-    congruence.
+  apply transpose_push_push_pop_reverse_right.
 Qed.
 
-Lemma transpose_push_pop_pop_reverse_middle vo1 v2 v3 :
-  unshift_var_opt_var
-    (unshift_var_var_opt (shift_var v2 v3) vo1)
-    (unshift_var v3 v2)
+Lemma transpose_push_pop_pop_reverse_middle v1 v2 v3 :
+  unshift_var
+    (unshift_var (shift_var v2 v3) v1) (unshift_var v3 v2)
   = unshift_var
-      (unshift_var_opt_var (unshift_var_var_opt v2 vo1) v3)
-      (unshift_var_opt_var vo1 v2).
+      (unshift_var (unshift_var v2 v1) v3)
+      (unshift_var v1 v2).
 Proof.
-  destruct vo1 as [v1|]; cbn; try easy.
-  rewrite transpose_push_push_pop_reverse_middle_aux; easy.
+  rewrite transpose_push_push_pop_reverse_middle; easy.
 Qed.
 
-Lemma transpose_push_pop_pop_reverse_right vo1 v2 v3 :
-  unshift_var_var_opt
-    (unshift_var v3 v2)
-    (unshift_var_var_opt (shift_var v2 v3) vo1)
-  = unshift_var_var_opt v3 (unshift_var_var_opt v2 vo1).
+Lemma transpose_push_pop_pop_reverse_right v1 v2 v3 :
+  unshift_var
+    (unshift_var v3 v2) (unshift_var (shift_var v2 v3) v1)
+  = unshift_var v3 (unshift_var v2 v1).
 Proof.
-  destruct vo1 as [v1|]; cbn; try easy.
-  rewrite transpose_pops_reverse_right; easy.
+  apply transpose_pops_reverse_right.
 Qed.
 
 (* In addition to the equalities between permutations, we
@@ -897,51 +747,18 @@ Qed.
    either direction is equivalent to doing nothing.
 *)
 
-Lemma transpose_reducing_push_pop_aux v1 v2 :
-  unshift_var v1 (shift_var v1 v2) = v2.
-Proof. case_vars v1 v2; easy. Qed.
-
-Lemma transpose_reducing_pop_push_aux v1 v2 :
+(* Moving an operation backwards over a
+   reducing pop and push *)
+Lemma transpose_op_reducing_pop_push v1 v2 :
   v1 <> v2 ->
   shift_var v1 (unshift_var v1 v2) = v2.
 Proof. case_vars v1 v2; easy. Qed.
 
-(* Moving a pop backwards over a reducing pop and push *)
-Lemma transpose_pop_reducing_pop_push v1 v2 :
-  v1 <> v2 ->
-  shift_var v1 (unshift_var_opt_var (Some v1) v2) = v2.
-Proof.
-  intros Hneq; cbn.
-  rewrite transpose_reducing_pop_push_aux by easy.
-  easy.
-Qed.
-
-(* Moving a pop backwards over a reducing push and pop *)
-Lemma transpose_pop_reducing_push_pop v1 v2 :
-  unshift_var_opt_var (Some v1) (shift_var v1 v2) = v2.
-Proof.
-  apply transpose_reducing_push_pop_aux.
-Qed.
-
-(* Moving a push forwards over a reducing pop and push *)
-Lemma transpose_push_reducing_pop_push v1 vo2 :
-  Some v1 <> vo2 ->
-  shift_var_opt (Some v1) (unshift_var_var_opt v1 vo2) = vo2.
-Proof.
-  intros Hneq.
-  destruct vo2; cbn; try easy.
-  rewrite transpose_reducing_pop_push_aux by congruence.
-  easy.
-Qed.
-
-(* Moving a push forwards over a reducing push and pop *)
-Lemma transpose_push_reducing_push_pop v1 vo2 :
-  unshift_var_var_opt v1 (shift_var_opt (Some v1) vo2) = vo2.
-Proof.
-  destruct vo2; cbn; try easy.
-  rewrite transpose_reducing_push_pop_aux by congruence.
-  easy.
-Qed.
+(* Moving an operation backwards over a
+   reducing push and pop *)
+Lemma transpose_op_reducing_push_pop v1 v2 :
+  unshift_var v1 (shift_var v1 v2) = v2.
+Proof. case_vars v1 v2; easy. Qed.
 
 (* [is_less_equal_var] is a total ordering *)
 
@@ -974,14 +791,13 @@ Definition is_less_equal_vars_transitive v1 v2 v3 :
   is_less_equal_vars v2 v3 = true ->
   is_less_equal_vars v1 v3 = true.
 Proof.
-  case_vars v1 v2; try easy.
-  - case_vars v2 v3; try rewrite Heql; easy.
-  - case_vars v2 v3; try rewrite Heql; try easy.
-    case_vars v1 v3; try easy.
-    + intros Heq1 Heq2.
-      apply is_less_than_label_opt_asymmetric in Heq2.
-      congruence.
-    + apply is_less_than_label_opt_transitive.
+  case_vars v1 v2; try easy;
+    case_vars v2 v3; try rewrite Heql; try easy.
+  case_vars v1 v3; try easy.
+  - intros Heq1 Heq2.
+    apply is_less_than_label_opt_asymmetric in Heq2.
+    congruence.
+  - apply is_less_than_label_opt_transitive.
 Qed.
 
 (* Orderings on shift and unshift *)
